src/axiomatic/TsoAtoP.v
@@ -1255,7 +1255,7 @@ Proof.
     esplits.
     { econs. econs; ss.
       - econs; ss.
-      - econs 5; ss.
+      - econs 6; ss.
     }
     econs; ss.
     econs; ss.
