src/promising/TsoPtoPF.v
@@ -96,7 +96,17 @@ Proof.
           - f_equal. apply Promises.set_unset.
             ii. subst. lia.
         }
-        { econs 5; eauto. inv STEP. econs; eauto. }
+        { econs 5; eauto. instantiate (1 := old_ts). instantiate (1 := vold).
+          inv STEP. exploit ExecUnit.read_wf; try exact OLD_MSG. i.
+          econs; eauto; ss.
+          - ii. eapply LATEST; eauto.
+            rewrite nth_error_app1 in MSG; ss.
+            eapply lt_le_trans. eauto.
+            inv WF. exploit WF0; eauto. i. inv x. ss. inv LOCAL.
+            repeat apply join_spec; viewtac.
+          - apply Memory.read_mon. ss.
+        }
+        { econs 6; eauto. inv STEP. econs; eauto. }
       * rewrite ? IdMap.add_add. eauto.
   - (* diff thread *)
     inv STEP. inv STEP1. inv STEP0. inv LOCAL0. inv MEM2. ss. subst.
@@ -142,7 +152,18 @@ Proof.
           - econs; ss.
           - apply Memory.get_msg_mon. ss.
         }
-        { econs 5; eauto. }
+        { econs 5; eauto. instantiate (1 := old_ts). instantiate (1 := vold).
+          inv STEP. exploit ExecUnit.read_wf; try exact OLD_MSG. i.
+          econs; eauto; ss.
+          - ii. eapply LATEST; eauto.
+            destruct (lt_dec ts (length mem1)).
+            { rewrite nth_error_app1 in MSG; ss. }
+            contradict n.
+            eapply Time.lt_le_trans; [apply TS2|].
+            inv WF. exploit WF0; try exact FIND; eauto. i. inv x. inv LOCAL. viewtac.
+          - apply Memory.read_mon. ss.
+        }
+        { econs 6; eauto. }
       * apply IdMap.add_add_diff. ss.
 Qed.
 
